{
 "cells": [
  {
   "cell_type": "markdown",
   "metadata": {},
   "source": [
    "# Chapter 4: Exercises Solutions"
   ]
  },
  {
   "cell_type": "markdown",
   "metadata": {},
   "source": [
    "1. Construct  $p_0(x),p_1(x),p_2(x),p_3(x)$, monic OPs\n",
    "   for the weight $\\sqrt{1-x^2}$ on $[-1,1]$.\n",
    "   \n",
    "   Hint: first compute $\\int_{-1}^1 x^k \\sqrt{1-x^2} {\\rm d} x$ for $0 ≤ k ≤ 2$\n",
    "   using a change-of-variables.\n",
    "\n",
    "Following the hint, we first calculate $\\int_{-1}^1 x^k\\sqrt{1-x^2}{\\rm d}x$. By symmetry, it's zero when $k$ is odd and double the integral on $[0,1]$ when $k$ is even. \n",
    "\n",
    "$$\n",
    "\\underbrace{\\int_0^1 x^k\\sqrt{1-x^2}{\\rm d}x}_{I_k}=_{x=\\sin t}\\underbrace{\\int_0^{\\pi/2}\\sin^k(t)\\cos^2(t){\\rm d}t}_{I_k}=\\underbrace{\\int_0^{\\pi/2}\\sin^k t{\\rm d}t}_{J_k}-\\underbrace{\\int_0^{\\pi/2}\\sin^{k+2}t{\\rm d}t}_{J_{k+2}}.\n",
    "$$\n",
    "\n",
    "Meanwhile, \n",
    "$$J_k=-\\int_0^{\\pi/2}\\sin^{k-1}t{\\rm d}(\\cos t)=_{\\text{integral by part}}(k-1)I_{k-2}.$$\n",
    "\n",
    "Putting the above 2 equations together, we have $I_k=(k-1)I_{k-2}-(k+1)I_k$, so $I_k=\\frac{k-1}{k+2}I_{k-2}$. Since $I_0=\\pi/4$, we have $I_k=\\frac{(k-1)!!}{(k+2)!!}\\frac{\\pi}{2}$ for positive even $k$. (Note that the denominator multiplies to 4, not to 2.) Keep in mind that the integral we want is double this value when $k$ is even.\n",
    "\n",
    "【Remark】Check the [beta function](https://en.wikipedia.org/wiki/Beta_function).\n",
    "\n",
    "Let $p_0(x)=1$, then $\\|p_0\\|^2=2I_0=\\pi/2$. We know from the 3-term recurrence that\n",
    "$$xp_0(x)=a_0p_0(x)+p_1(x)$$\n",
    "where\n",
    "$$\n",
    "a_0=\\frac{⟨ p_0,xp_0⟩}{\\|p_0\\|^2}=0.$$\n",
    "Thus $p_1(x)=x$ and $\\|p_1\\|^2=2I_2=\\pi/8$.\n",
    "From\n",
    "$$xp_1(x)=c_0p_0(x)+a_1p_1(x)+p_2(x)$$\n",
    "we have\n",
    "$$c_0=\\frac{⟨ p_0,xp_1⟩}{\\|p_0\\|^2}=2I_2/2I_0=1/4$$\n",
    "$$a_1=\\frac{⟨ p_1,xp_1⟩}{\\|p_1\\|^2}=0$$\n",
    "$$p_2(x)=xp_1(x)-c_0-a_1p_1(x)=x^2-1/4$$\n",
    "$$\\|p_2\\|^2=2I_4-I_2+1/8I_0=\\pi/32$$\n",
    "Finally, from\n",
    "$$xp_2(x)=c_1p_1(x)+a_2p_2(x)+p_3(x)$$\n",
    "we have\n",
    "$$c_1=\\frac{⟨ p_1,xp_2⟩}{\\|p_1\\|^2}=(2I_4-1/2I_2)/(\\pi/8)=1/4$$\n",
    "$$a_2=\\frac{⟨ p_2,xp_2⟩}{\\|p_2\\|^2}=0$$\n",
    "$$p_3(x)=xp_2(x)-c_1p_1(x)-a_2p_2(x)=x^3-1/2x$$\n"
   ]
  },
  {
   "cell_type": "markdown",
   "metadata": {},
   "source": [
    "2. Let $w(x)$ be a weight function on $x \\in [-b, b]$, $b > 0$ satisfying $w(-x) = w(x)$. Show that $a_n = 0$, $n \\geq 0$ and conclude that $a_n = 0$ for the Chebyshev polynomials $\\lbrace T_n \\rbrace$ and the ultraspherical polynomials $\\lbrace C_n^{(\\lambda)}\\rbrace$.\n",
    "    \n",
    "    Hint: first show that the OPs $p_{2n}(x)$ are even and $p_{2n+1}(x)$ are odd."
   ]
  },
  {
   "cell_type": "markdown",
   "metadata": {},
   "source": [
    "Recall that \n",
    "$$\n",
    "a_n = \\frac{\\langle xp_n, p_n\\rangle}{\\langle p_n, p_n\\rangle},\n",
    "$$\n",
    "where\n",
    "$$\n",
    "\\langle f, g \\rangle = \\int_{-b}^{b} f(x)g(x)w(x)\\,{\\rm d}x.\n",
    "$$\n",
    "The inner product is zero if the integrand is odd. \n",
    "Moreover an even function times an odd function is odd and\n",
    "an odd function times an odd fuction is even.\n",
    "Note that $p_0(x)$ and $w(x)$ are even and $x$ is odd. \n",
    "\n",
    "We see that $a_0$ is zero\n",
    "$$\n",
    "⟨p_0,x p_0(x)⟩ = p_0^2\\int_{-b}^b x w(x) {\\rm d} x = 0\n",
    "$$\n",
    "since $xw(x)$ is odd,\n",
    "which shows that\n",
    "$$\n",
    "p_1(x) = xp_0(x)/b_0\n",
    "$$\n",
    "is odd. We now proceed by induction. Assume that $p_{2n}$ is even and $p_{2n-1}$ is odd.\n",
    "We have:\n",
    "$$\n",
    "⟨p_{2n},x p_{2n}(x)⟩ = \\int_{-b}^b x w(x) p_{2n}(x)^2 {\\rm d} x = 0\n",
    "$$\n",
    "since $x w(x) p_{2n}(x)^2$ is odd, therefore $a_{2n} = 0$.\n",
    "Thus from\n",
    "$$\n",
    "p_{2n+1}(x) = (x p_{2n}(x)- c_{2n-1} p_{2n-1}(x)) / b_{2n} \n",
    "$$\n",
    "we see that $p_{2n+1}$ is odd. Then\n",
    "$$\n",
    "⟨p_{2n+1},x p_{2n+1}(x)⟩ = \\int_{-b}^b x w(x) p_{2n+1}(x)^2 {\\rm d} x = 0\n",
    "$$\n",
    "since $x w(x) p_{2n+1}(x)^2$ is odd, therefore $a_{2n+1} = 0$.\n",
    "and hence\n",
    "$$\n",
    "p_{2n+2}(x) = (x p_{2n+1}(x)- c_{2n} p_{2n}(x)) / b_{2n+1} \n",
    "$$\n",
    "is even.\n",
    "\n",
    "For the Chebyshev polynomials and the ultraspherical polynomials, $b = 1$ and the weight functions are even; therefore $a_n = 0$."
   ]
  },
  {
   "cell_type": "markdown",
   "metadata": {},
   "source": [
    "3. "
   ]
  },
  {
   "cell_type": "markdown",
   "metadata": {},
   "source": [
    "\n",
    "\n",
    "4. Ask question about Bandwidths of combination of conversion matrices\n",
    "\n",
    "5. Ask question about differentiation matrix when we don't change basis"
   ]
  },
  {
   "cell_type": "markdown",
   "metadata": {},
   "source": [
    "Look at Chapter 4 exercises, draft"
   ]
  },
  {
   "cell_type": "markdown",
   "metadata": {},
   "source": [
    "Try to do the analogue of the Hermite exercises below for Laguerre"
   ]
  },
  {
   "cell_type": "markdown",
   "metadata": {},
   "source": [
    "**Problem 2.3 (B)**\n",
    "Consider orthogonal polynomials with respect to $\\sqrt{1-x^2}$ on $[-1,1]$ with the\n",
    "normalisation\n",
    "$$\n",
    "U_n(x) = 2^n x^n + O(x^{n-1})\n",
    "$$\n",
    "Prove that\n",
    "$$\n",
    "U_n(\\cos θ) = {\\sin(n+1) θ \\over \\sin θ}\n",
    "$$\n",
    "\n",
    "**SOLUTION**\n",
    "\n",
    "We need to verify:\n",
    "1. graded polynomials\n",
    "2. orthogonal w.r.t. $\\sqrt{1-x^2}$ on $[-1,1]$, and\n",
    "3. have the leading coefficient $2^n$.\n",
    "\n",
    "(2) follows under a change of variables\n",
    "$$\\int_{-1}^1U_n(x)U_m(x)\\sqrt{1-x^2}{\\rm d}x=\\int_0^{\\pi}U_n(\\cos\\theta)U_m(\\cos\\theta)\\sin^2\\theta{\\rm d}\\theta=\\int_0^{\\pi}\\sin(n+1)\\theta\\sin(m+1)\\theta{\\rm d}\\theta=\\frac{\\pi}{2}\\delta_{mn}$$\n",
    "where the last step is a result from Fourier theories.\n",
    "\n",
    "To see that they are graded we use the fact that\n",
    "$$xU_n(x)=\\frac{\\cos\\theta\\sin(n+1)\\theta}{\\sin\\theta}=\\frac{\\sin (n+2)\\theta+\\sin n\\theta}{2\\sin\\theta}$$\n",
    "In other words $2xU_n(x)=U_{n+1}(x)+U_{n-1}(x)$. Since each time we multiply by $2x$ and $U_0(x)=1$ we have\n",
    "$$U_n(x) = 2^n x^n + O(x^{n-1})$$\n",
    "which also proves (3)."
   ]
  },
  {
   "cell_type": "markdown",
   "metadata": {},
   "source": [
    "**Problem 2.4 (B)** Show that\n",
    "$$\n",
    "\\begin{align*}\n",
    "x U_0(x) &= U_1(x)/2 \\\\\n",
    "x U_n(x) &= {U_{n-1}(x) \\over 2} + {U_{n+1}(x) \\over 2}.\n",
    "\\end{align*}\n",
    "$$\n",
    "\n",
    "**SOLUTION**\n",
    "\n",
    "The first result is trivial.\n",
    "\n",
    "To get the second result, recall that\n",
    "$$U_n(\\cos\\theta)=\\cos\\theta U_{n-1}(\\cos\\theta)+\\cos n\\theta$$\n",
    "and\n",
    "$$\\cos n\\theta=\\cos\\theta\\cos(n-1)\\theta-(1-\\cos^2\\theta)U_{n-2}(\\cos\\theta).$$\n",
    "\n",
    "The first equation gives $\\cos n\\theta$ in terms of $U_n$ and $U_{n-1}$. Substitute the result into the second equation to get\n",
    "$$U_n(x)-xU_{n-1}(x)=x(U_{n-1}(x)-xU_{n-2}(x))-(1-x^2)U_{n-2}(x)$$\n",
    "which reduces to the desired recurrence."
   ]
  },
  {
   "cell_type": "markdown",
   "metadata": {},
   "source": [
    "**Problem 3.1 (B)** Consider Hermite polynomials orthogonal with respect to the weight $\\exp(-x^2)$ on $ℝ$\n",
    "with the normalisation\n",
    "$$\n",
    "H_n(x) = 2^n x^n + O(x^{n-1}).\n",
    "$$\n",
    "Prove the Rodrigues formula\n",
    "$$\n",
    "H_n(x) = (-1)^n \\exp(x^2) {{\\rm d}^n \\over {\\rm d}x^n} \\exp(-x^2)\n",
    "$$\n",
    "\n",
    "**SOLUTION**\n",
    "Define\n",
    "$$\n",
    "p_n(x) := (-1)^n \\exp(x^2) {{\\rm d}^n \\over {\\rm d}x^n} \\exp(-x^2)\n",
    "$$\n",
    "\n",
    "We need to verify that $p_n$\n",
    "1. are graded polynomials\n",
    "2. are orthogonal to all lower degree polynomials on $\\mathbb{R}$, and\n",
    "3. have the right leading coefficient $2^n$.\n",
    "\n",
    "Comparing the Rodrigues formula for $n$ and $n-1$, we find that \n",
    "$$\n",
    "(-1)^n\\exp(-x^2)p_n(x)={{\\rm d} \\over {\\rm d}x}\\left((-1)^{n-1}\\exp(-x^2)p_{n-1}(x)\\right)\n",
    "$$\n",
    "which reduces to\n",
    "$$p_n(x)=2xp_{n-1}(x)-p_{n-1}'(x).$$\n",
    "\n",
    "(1) and (3) then follows from induction since $p_0(x)=1$.\n",
    "\n",
    "(2) follows by integration by parts. If $r_m$ is any degree $m<n$ polynomial we have:\n",
    "$$\n",
    "\\begin{align*}\n",
    "\\int_{-∞}^∞ p_n(x)r_m(x)\\exp(-x^2){\\rm d}x&=\\int_{-∞}^∞{{\\rm d}^n \\over {\\rm d}x^n} \\exp(-x^2)r(x){\\rm d}x = -\\int_{-∞}^∞{{\\rm d}^{n-1} \\over {\\rm d}x^{n-1}} \\exp(-x^2)r'(x){\\rm d}x\\\\\n",
    "&=⋯\\text{integration by parts $n$ times}…=(-1)^n\\int_{-∞}^∞ \\exp(-x^2)r_m^{(n)}(x)=0\n",
    "\\end{align*}\n",
    "$$\n",
    "Thus $p_n(x) = H_n(x)$ by uniqueness.\n",
    "\n",
    "**Problem 3.2 (C)** What are $k_n^{(1)}$ and $k_n^{(2)}$ such that\n",
    "$$\n",
    "H_n(x) = 2^n x^n + k_n^{(1)} x^{n-1} + k_n^{(2)} x^{n-2} + O(x^{n-3})\n",
    "$$\n",
    "\n",
    "**SOLUTION**\n",
    "\n",
    "From Problem 3.1,\n",
    "$$H_n(x)=2xH_{n-1}(x)-H_{n-1}'(x).$$\n",
    "Thus we have\n",
    "$$k_n^{(1)}=2k_{n-1}^{(1)}$$\n",
    "$$k_n^{(2)}=2k_{n-1}^{(2)}-(n-1)2^{n-1}$$\n",
    "\n",
    "Since $k_0^{(1)}=0$, we have $k_n^{(1)}=0$. For the second recurrence, divide both sides by $2^n$:\n",
    "$$2^{-n}k_n^{(2)}=2^{-(n-1)}k_{n-1}^{(2)}-\\frac{n-1}{2}$$\n",
    "Since $k_0^{(2)}=0$, we have $2^{-n}k_n^{(2)}=-\\frac{1+\\cdots+(n-1)}{2}=-\\frac{n(n-1)}{4}$, so $k_n^{(2)}=-n(n-1)2^{n-2}$.\n",
    "\n",
    "**Problem 3.3 (B)** Deduce the 3-term recurrence relationship for $H_n(x)$.\n",
    "\n",
    "**SOLUTION**\n",
    "\n",
    "Our goal is to find $a_n$, $b_n$ and $c_n$ such that\n",
    "$$xH_n(x)=c_{n-1}H_{n-1}(x)+a_nH_n(x)+b_nH_{n+1}(x).$$\n",
    "Compare the 3 leading coefficients on both sides and use the results from Problem 3.1 and Problem 3.2:\n",
    "$$\n",
    "2^n=0+0+b_n2^{n+1}\n",
    "$$\n",
    "$$\n",
    "0=0+a_n2^n+0\n",
    "$$\n",
    "$$\n",
    "n(n-1)2^{n-2}=c_{n-1}2^{n-1}+0+b_n(n+1)n2^{n-1}\n",
    "$$\n",
    "Thus we have $b_n=1/2$, $a_n=0$ and $c_{n-1}=n$.\n"
   ]
  },
  {
   "cell_type": "code",
   "execution_count": null,
   "metadata": {},
   "outputs": [],
   "source": []
  }
 ],
 "metadata": {
  "kernelspec": {
   "display_name": "Julia 1.8.3",
   "language": "julia",
   "name": "julia-1.8"
  },
  "language_info": {
   "file_extension": ".jl",
   "mimetype": "application/julia",
   "name": "julia",
   "version": "1.8.3"
  }
 },
 "nbformat": 4,
 "nbformat_minor": 4
}
