{
 "cells": [
  {
   "cell_type": "markdown",
   "metadata": {},
   "source": [
    "Try to do the analogue of the Hermite exercises below for Laguerre"
   ]
  },
  {
   "cell_type": "markdown",
   "metadata": {},
   "source": [
    "**Problem 3.1 (B)** Consider Hermite polynomials orthogonal with respect to the weight $\\exp(-x^2)$ on $ℝ$\n",
    "with the normalisation\n",
    "$$\n",
    "H_n(x) = 2^n x^n + O(x^{n-1}).\n",
    "$$\n",
    "Prove the Rodrigues formula\n",
    "$$\n",
    "H_n(x) = (-1)^n \\exp(x^2) {{\\rm d}^n \\over {\\rm d}x^n} \\exp(-x^2)\n",
    "$$\n",
    "\n",
    "**SOLUTION**\n",
    "Define\n",
    "$$\n",
    "p_n(x) := (-1)^n \\exp(x^2) {{\\rm d}^n \\over {\\rm d}x^n} \\exp(-x^2)\n",
    "$$\n",
    "\n",
    "We need to verify that $p_n$\n",
    "1. are graded polynomials\n",
    "2. are orthogonal to all lower degree polynomials on $\\mathbb{R}$, and\n",
    "3. have the right leading coefficient $2^n$.\n",
    "\n",
    "Comparing the Rodrigues formula for $n$ and $n-1$, we find that \n",
    "$$\n",
    "(-1)^n\\exp(-x^2)p_n(x)={{\\rm d} \\over {\\rm d}x}\\left((-1)^{n-1}\\exp(-x^2)p_{n-1}(x)\\right)\n",
    "$$\n",
    "which reduces to\n",
    "$$p_n(x)=2xp_{n-1}(x)-p_{n-1}'(x).$$\n",
    "\n",
    "(1) and (3) then follows from induction since $p_0(x)=1$.\n",
    "\n",
    "(2) follows by integration by parts. If $r_m$ is any degree $m<n$ polynomial we have:\n",
    "$$\n",
    "\\begin{align*}\n",
    "\\int_{-∞}^∞ p_n(x)r_m(x)\\exp(-x^2){\\rm d}x&=\\int_{-∞}^∞{{\\rm d}^n \\over {\\rm d}x^n} \\exp(-x^2)r(x){\\rm d}x = -\\int_{-∞}^∞{{\\rm d}^{n-1} \\over {\\rm d}x^{n-1}} \\exp(-x^2)r'(x){\\rm d}x\\\\\n",
    "&=⋯\\text{integration by parts $n$ times}…=(-1)^n\\int_{-∞}^∞ \\exp(-x^2)r_m^{(n)}(x)=0\n",
    "\\end{align*}\n",
    "$$\n",
    "Thus $p_n(x) = H_n(x)$ by uniqueness.\n",
    "\n",
    "**Problem 3.2 (C)** What are $k_n^{(1)}$ and $k_n^{(2)}$ such that\n",
    "$$\n",
    "H_n(x) = 2^n x^n + k_n^{(1)} x^{n-1} + k_n^{(2)} x^{n-2} + O(x^{n-3})\n",
    "$$\n",
    "\n",
    "**SOLUTION**\n",
    "\n",
    "From Problem 3.1,\n",
    "$$H_n(x)=2xH_{n-1}(x)-H_{n-1}'(x).$$\n",
    "Thus we have\n",
    "$$k_n^{(1)}=2k_{n-1}^{(1)}$$\n",
    "$$k_n^{(2)}=2k_{n-1}^{(2)}-(n-1)2^{n-1}$$\n",
    "\n",
    "Since $k_0^{(1)}=0$, we have $k_n^{(1)}=0$. For the second recurrence, divide both sides by $2^n$:\n",
    "$$2^{-n}k_n^{(2)}=2^{-(n-1)}k_{n-1}^{(2)}-\\frac{n-1}{2}$$\n",
    "Since $k_0^{(2)}=0$, we have $2^{-n}k_n^{(2)}=-\\frac{1+\\cdots+(n-1)}{2}=-\\frac{n(n-1)}{4}$, so $k_n^{(2)}=-n(n-1)2^{n-2}$.\n",
    "\n",
    "**Problem 3.3 (B)** Deduce the 3-term recurrence relationship for $H_n(x)$.\n",
    "\n",
    "**SOLUTION**\n",
    "\n",
    "Our goal is to find $a_n$, $b_n$ and $c_n$ such that\n",
    "$$xH_n(x)=c_{n-1}H_{n-1}(x)+a_nH_n(x)+b_nH_{n+1}(x).$$\n",
    "Compare the 3 leading coefficients on both sides and use the results from Problem 3.1 and Problem 3.2:\n",
    "$$\n",
    "2^n=0+0+b_n2^{n+1}\n",
    "$$\n",
    "$$\n",
    "0=0+a_n2^n+0\n",
    "$$\n",
    "$$\n",
    "n(n-1)2^{n-2}=c_{n-1}2^{n-1}+0+b_n(n+1)n2^{n-1}\n",
    "$$\n",
    "Thus we have $b_n=1/2$, $a_n=0$ and $c_{n-1}=n$.\n"
   ]
  }
 ],
 "metadata": {
  "kernelspec": {
   "display_name": "Julia 1.8.3",
   "language": "julia",
   "name": "julia-1.8"
  },
  "language_info": {
   "file_extension": ".jl",
   "mimetype": "application/julia",
   "name": "julia",
   "version": "1.8.3"
  }
 },
 "nbformat": 4,
 "nbformat_minor": 4
}
